cleanup Hedge library and remove List theorems

VerifiedFilter/Std/List.lean
@@ -3,19 +3,6 @@ import Mathlib.Tactic.RewriteSearch
 
 namespace List
 
-abbrev ElemOf {α: Type} (xs: List α) := { y: α // y ∈ xs }
-
-def ElemOf.mk {α: Type} (y: α) (xs: List α) (property : y ∈ xs) : ElemOf xs :=
-  (Subtype.mk y property)
-
-def ElemOf.self {α: Type} (x: α) : ElemOf [x] :=
-  (Subtype.mk x (by simp only [mem_cons, not_mem_nil, or_false]))
-
-def ElemOf.selfs {α: Type} (xs: List α) : List (ElemOf xs) :=
-  map (fun x =>
-    ElemOf.mk x.val xs x.property
-  ) xs.attach
-
 def snoc (xs: List α) (x: α) :=
   xs ++ [x]
 
@@ -27,52 +14,6 @@ theorem list_elem_lt [SizeOf α] {xs: List α} (h: x ∈ xs): sizeOf x ≤ sizeO
   | tail _ _ ih =>
     apply Nat.le_trans ih
     simp +arith
-
-theorem list_foldl_attach {f: β → α → β} {init: β} {xs: List α}:
-  List.foldl (fun res ⟨x, _hx⟩ => f res x) init (List.attach xs)
-  = List.foldl f init xs := by
-  simp only [foldl_subtype, unattach_attach]
-
-theorem list_splitAt_n: xs = (List.splitAt n xs).1 ++ (List.splitAt n xs).2 := by
-  simp only [List.splitAt_eq, List.take_append_drop]
-
-theorem list_splitAt_fst_take: (List.splitAt n xs).1 = take n xs := by
-  simp only [List.splitAt_eq]
-
-theorem list_splitAt_snd_drop: (List.splitAt n xs).2 = drop n xs := by
-  simp only [List.splitAt_eq]
-
-theorem list_take_drop_n (n: Nat) (xs: List α): xs = List.take n xs ++ List.drop n xs := by
-  simp only [List.take_append_drop]
-
-theorem list_sizeOf_prepend [SizeOf α] (xs ys: List α):
-  sizeOf xs <= sizeOf (ys ++ xs) := by
-  induction ys with
-  | nil =>
-    simp only [List.nil_append, Nat.le_refl]
-  | cons y ys ih =>
-    simp +arith only [List.cons_append, List.cons.sizeOf_spec]
-    omega
-
-theorem list_sizeOf_insert [SizeOf α] (xs ys: List α):
-  sizeOf (y::xs ++ ys) = sizeOf (xs ++ y::ys) := by
-  induction xs with
-  | nil =>
-    simp [List.cons.sizeOf_spec]
-  | cons x xs ih =>
-    simp [List.cons.sizeOf_spec]
-    rw [<- ih]
-    simp +arith [List.cons.sizeOf_spec]
-
-theorem list_sizeOf_append [SizeOf α] (xs ys: List α):
-  sizeOf xs <= sizeOf (xs ++ ys) := by
-  induction ys with
-  | nil =>
-    simp only [append_nil, Nat.le_refl]
-  | cons y ys ih =>
-    rw [<- list_sizeOf_insert]
-    simp +arith only [List.cons_append, List.cons.sizeOf_spec]
-    omega
 
 theorem list_sizeOf_cons [SizeOf α] (xs ys: List α):
   sizeOf xs < sizeOf (y::ys ++ xs) := by
@@ -101,53 +42,10 @@ theorem list_sizeOf_lt_cons_lt [SizeOf α] (x: α) {ys xs: List α} (h_lt: sizeO
   simp [cons.sizeOf_spec]
   exact Nat.lt_add_left (1 + sizeOf x) h_lt
 
-theorem list_length_neq_take {n: Nat} {xs: List α}:
-  ¬List.take n xs = xs → (List.take n xs).length < xs.length := by
-  intro h
-  fun_induction List.take
-  case case1 xs =>
-    simp
-    cases xs with
-    | nil =>
-      simp at h
-    | cons x xs =>
-      simp
-  case case2 =>
-    simp at h
-  case case3 n x xs h' =>
-    simp at h
-    have h' := h' h
-    simp only [length_cons]
-    omega
-
-theorem list_length_neq_drop {n: Nat} {xs: List α}:
-  ¬List.drop n xs = xs → (List.drop n xs).length < xs.length := by
-  intro h
-  induction n with
-  | zero =>
-    simp at h
-  | succ n =>
-    cases xs with
-    | nil =>
-      simp at h
-    | cons x xs =>
-      simp
-      omega
-
 theorem list_length_drop_lt_cons {n: Nat} {xs: List α}:
   (List.drop n xs).length < (x :: xs).length := by
   simp only [length_drop, length_cons]
   omega
-
-theorem list_sizeOf_slice [SizeOf α] (xs ys zs: List α):
-  sizeOf ys <= sizeOf (xs ++ (ys ++ zs)) := by
-  induction xs with
-  | nil =>
-    simp only [nil_append]
-    apply list_sizeOf_append ys zs
-  | cons x xs ih =>
-    simp [List.cons.sizeOf_spec]
-    omega
 
 theorem list_drop_exists (n: Nat) (xs: List α): ∃ ys, xs = ys ++ (List.drop n xs) := by
   cases n with
@@ -166,126 +64,8 @@ theorem list_drop_exists (n: Nat) (xs: List α): ∃ ys, xs = ys ++ (List.drop n
       congr
       simp only [take_append_drop]
 
-theorem list_self_neq_cons_append:
-  xs ≠ y :: (ys ++ xs) := by
-  intro h
-  rw [←List.cons_append] at h
-  rw [List.self_eq_append_left] at h
-  nomatch h
 
-theorem list_drop_neq_cons:
-  List.drop n xs ≠ x :: xs := by
-  have h := list_drop_exists n xs
-  cases h with
-  | intro ys h =>
-  nth_rewrite 2 [h]
-  simp
-  exact list_self_neq_cons_append (xs := drop n xs) (y := x) (ys := ys)
-
-theorem list_sizeOf_take_drop_le [SizeOf α] (xs: List α):
-  sizeOf (List.take t (List.drop d xs)) <= sizeOf xs := by
-  induction xs generalizing t d with
-  | nil =>
-    simp
-  | cons x xs ih =>
-    simp only [List.cons.sizeOf_spec]
-    cases d with
-    | zero =>
-      simp
-      cases t with
-      | zero =>
-        simp
-        omega
-      | succ t =>
-        simp
-        have ih' := @ih t 0
-        simp at ih'
-        assumption
-    | succ d =>
-      simp
-      have ih' := @ih t d
-      omega
-
-theorem list_take_n_nil {n: Nat} {α: Type}:
-  @List.take α n [] = [] := by
-  simp
-
-theorem list_infix_take_is_infix:
-  List.IsInfix xs (List.take n ys) →
-  List.IsInfix xs ys := by
-  intro h
-  have hys := List.infix_append [] (List.take n ys) (List.drop n ys)
-  simp at hys
-  apply List.IsInfix.trans h hys
-
-theorem list_infix_drop_is_infix:
-  List.IsInfix xs (List.drop n ys) →
-  List.IsInfix xs ys := by
-  intro h
-  have hys := List.infix_append (List.take n ys) (List.drop n ys) []
-  simp at hys
-  apply List.IsInfix.trans h hys
-
-theorem list_infix_def {xs ys: List α}:
-  List.IsInfix xs ys →
-  ∃ xs1 xs2, xs1 ++ xs ++ xs2 = ys := by
-  intro h
-  obtain ⟨xs1, h⟩ := h
-  obtain ⟨xs2, h⟩ := h
-  exists xs1
-  exists xs2
-
-abbrev InfixOf {α: Type} (xs: List α) := { ys: List α // List.IsInfix ys xs }
-
-def InfixOf.mk {α: Type} {xs: List α} (ys: List α) (property : List.IsInfix ys xs) : InfixOf xs :=
-  (Subtype.mk ys property)
-
-def InfixOf.self (xs: List α): InfixOf xs :=
-  Subtype.mk xs (by simp only [List.infix_rfl])
-
-theorem list_infixof_take_is_infix {xs: List α} (ys: InfixOf (List.take n xs)):
-  List.IsInfix ys.val xs := by
-  obtain ⟨ys, hys⟩ := ys
-  simp
-  have h1 := list_infix_take_is_infix hys
-  assumption
-
-theorem list_infixof_drop_is_infix {xs: List α} (ys: InfixOf (List.drop n xs)):
-  List.IsInfix ys.val xs := by
-  obtain ⟨ys, hys⟩ := ys
-  simp
-  have h1 := list_infix_drop_is_infix hys
-  assumption
-
-theorem list_infix_is_leq_sizeOf {α: Type} [SizeOf α] {xs ys: List α}:
-  List.IsInfix xs ys →
-  sizeOf xs <= sizeOf ys := by
-  intro h
-  have h' := List.list_infix_def h
-  obtain ⟨xs1, xs2, h'⟩ := h'
-  rw [<- h']
-  have hh2 := List.list_sizeOf_append (xs1 ++ xs) xs2
-  have hh1 := List.list_sizeOf_prepend xs xs1
-  apply Nat.le_trans hh1 hh2
-
-theorem list_take_eq_self_iff (x : List α) {n : Nat} : x.take n = x ↔ x.length ≤ n :=
-  ⟨fun h ↦ by rw [← h]; simp; omega, take_of_length_le⟩
-
-theorem list_elemof_take_is_elem {xs: List α} (y: List.ElemOf (List.take n xs)):
-  y.val ∈ xs := by
-  obtain ⟨y, hy⟩ := y
-  simp only
-  rw [list_take_drop_n n xs]
-  rw [List.mem_append]
-  exact Or.inl hy
-
-theorem list_elemof_drop_is_elem {xs: List α} (y: List.ElemOf (List.drop n xs)):
-  y.val ∈ xs := by
-  obtain ⟨y, hy⟩ := y
-  simp only
-  rw [list_take_drop_n n xs]
-  rw [List.mem_append]
-  exact Or.inr hy
+-- interleaves
 
 def interleaves (xs: List α) (acc: List (List α × List α) := [([], [])])
   : List (List α × List α) := match xs with
